-- ğ•‹ğ• ğ•ğ•’ğ•« ğ”¾ğ• ğ•ğ•–ğ•¤ ğ•„ğ•’ğ•¤ğ•”ğ•’ğ•£ğ•–ğ•Ÿğ•™ğ•’ğ•¤


module plfa_decidable where

import Relation.Binary.PropositionalEquality as Eq
open Eq using (_â‰¡_; refl)
open Eq.â‰¡-Reasoning
open import plfa_naturals using (â„•; zero; suc; _âˆ¸_)
open import Data.Product using (_Ã—_) renaming (_,_ to âŸ¨_,_âŸ©)
open import Data.Empty using (âŠ¥; âŠ¥-elim)
open import plfa_negation using (Â¬_; Â¬Â¬-intro; contraposition)
open import plfa_connectives using (_âŠ_; injâ‚; injâ‚‚;
                                    âŠ¤; tt)
open import plfa_relations using (_â‰¤_; zâ‰¤n; sâ‰¤s;
                                  _<_; z<s; s<s)
open import plfa_isomorphism using (_â‡”_; _âˆ˜_)

data Bool : Set where
  true  : Bool
  false : Bool

infix 4 _â‰¤áµ‡_

_â‰¤áµ‡_ : â„• â†’ â„• â†’ Bool
zero  â‰¤áµ‡ n     = true
suc m â‰¤áµ‡ zero  = false
suc m â‰¤áµ‡ suc n = m â‰¤áµ‡ n

T : Bool â†’ Set
T true  = âŠ¤
T false = âŠ¥

Tâ†’â‰¡ : âˆ€ (b : Bool) â†’ T b â†’ b â‰¡ true
Tâ†’â‰¡ true tt   =  refl
Tâ†’â‰¡ false ()

â‰¡â†’T : âˆ€ {b : Bool} â†’ b â‰¡ true â†’ T b
â‰¡â†’T refl  =  tt

â‰¤áµ‡â†’â‰¤ : âˆ€ (m n : â„•) â†’ T (m â‰¤áµ‡ n) â†’ m â‰¤ n
â‰¤áµ‡â†’â‰¤ zero     n   tt = zâ‰¤n
â‰¤áµ‡â†’â‰¤ (suc m) zero ()
â‰¤áµ‡â†’â‰¤ (suc m) (suc n) t = sâ‰¤s (â‰¤áµ‡â†’â‰¤ m n t)

â‰¤â†’â‰¤áµ‡ : âˆ€ {m n : â„•} â†’ m â‰¤ n â†’ T (m â‰¤áµ‡ n)
â‰¤â†’â‰¤áµ‡ zâ‰¤n       = tt
â‰¤â†’â‰¤áµ‡ (sâ‰¤s mâ‰¤n) = â‰¤â†’â‰¤áµ‡ mâ‰¤n

data Dec (A : Set) : Set where
  yes :   A â†’ Dec A
  no  : Â¬ A â†’ Dec A

Â¬sâ‰¤z : âˆ€ {m : â„•} â†’ Â¬ (suc m â‰¤ zero)
Â¬sâ‰¤z ()

Â¬sâ‰¤s : âˆ€ {m n : â„•} â†’ Â¬ (m â‰¤ n) â†’ Â¬ (suc m â‰¤ suc n)
Â¬sâ‰¤s Â¬mâ‰¤n (sâ‰¤s mâ‰¤n) = Â¬mâ‰¤n mâ‰¤n

_â‰¤?_ : âˆ€ (m n : â„•) â†’ Dec (m â‰¤ n)
zero  â‰¤? n                   =  yes zâ‰¤n
suc m â‰¤? zero                =  no Â¬sâ‰¤z
suc m â‰¤? suc n with m â‰¤? n
...               | yes mâ‰¤n  =  yes (sâ‰¤s mâ‰¤n)
...               | no Â¬mâ‰¤n  =  no  (Â¬sâ‰¤s Â¬mâ‰¤n)

Â¬n<z : âˆ€ {n : â„•} â†’ Â¬ (n < zero)
Â¬n<z ()

Â¬s<s : âˆ€ {m n : â„•} â†’ Â¬ (m < n) â†’ Â¬ (suc m < suc n)
Â¬s<s Â¬m<n (s<s m<n) = Â¬m<n m<n

_<?_ : âˆ€ (m n : â„•) â†’ Dec (m < n)
zero <? zero = no Â¬n<z
zero <? suc m = yes z<s
suc n <? zero = no Â¬n<z
suc n <? suc m with n <? m
...             | yes n<m  = yes (s<s n<m)
...             | no  Â¬n<m = no (Â¬s<s Â¬n<m)

Â¬zâ‰¡sn : âˆ€ {n : â„•} â†’ Â¬ (zero â‰¡ suc n)
Â¬zâ‰¡sn ()

Â¬snâ‰¡z : âˆ€ {n : â„•} â†’ Â¬ (suc n â‰¡ zero)
Â¬snâ‰¡z ()

pred-â‰¡ : âˆ€ {m n : â„•} â†’ suc m â‰¡ suc n â†’ m â‰¡ n
pred-â‰¡ = Eq.cong (_âˆ¸ 1)

Â¬nâ‰¡mâ†’Â¬snâ‰¡sm : âˆ€ {n m : â„•} â†’ (Â¬ (n â‰¡ m)) â†’ (Â¬ ((suc n) â‰¡ (suc m)))
Â¬nâ‰¡mâ†’Â¬snâ‰¡sm nâ‰¢m = Î» { snâ‰¡sm  â†’ nâ‰¢m ((pred-â‰¡ snâ‰¡sm))}

_â‰¡â„•?_ : âˆ€ (m n : â„•) â†’ Dec (m â‰¡ n)
zero â‰¡â„•? zero = yes refl
zero â‰¡â„•? suc n = no Â¬zâ‰¡sn
suc m â‰¡â„•? zero = no Â¬snâ‰¡z
suc m â‰¡â„•? suc n with m â‰¡â„•? n
...              | yes nâ‰¡m = yes (Eq.cong suc nâ‰¡m)
...              | no  nâ‰¢m = no (Â¬nâ‰¡mâ†’Â¬snâ‰¡sm nâ‰¢m)

_â‰¤?â€²_ : âˆ€ (m n : â„•) â†’ Dec (m â‰¤ n)
m â‰¤?â€² n with m â‰¤áµ‡ n | â‰¤áµ‡â†’â‰¤ m n | â‰¤â†’â‰¤áµ‡ {m} {n}
...        | true   | p        | _            = yes (p tt)
...        | false  | _        | Â¬p           = no Â¬p



âŒŠ_âŒ‹ : {A : Set} â†’ Dec A â†’ Bool
âŒŠ yes a âŒ‹ = true
âŒŠ no Â¬a âŒ‹ = false

_â‰¤áµ‡Â´_ : â„• â†’ â„• â†’ Bool
_â‰¤áµ‡Â´_ m n = âŒŠ m â‰¤? n âŒ‹

toWitness : âˆ€ {A : Set} {D : Dec A} â†’ T âŒŠ D âŒ‹ â†’ A
toWitness {A} {yes x} tt  =  x
toWitness {A} {no Â¬x} ()

fromWitness : âˆ€ {A : Set} {D : Dec A} â†’ A â†’ T âŒŠ D âŒ‹
fromWitness {A} {yes x} _  =  tt
fromWitness {A} {no Â¬x} x  =  Â¬x x

â‰¤áµ‡Â´â†’â‰¤ : âˆ€ {m n : â„•} â†’ T (m â‰¤áµ‡Â´ n) â†’ m â‰¤ n
â‰¤áµ‡Â´â†’â‰¤  =  toWitness

â‰¤â†’â‰¤áµ‡Â´ : âˆ€ {m n : â„•} â†’ m â‰¤ n â†’ T (m â‰¤áµ‡Â´ n)
â‰¤â†’â‰¤áµ‡Â´  =  fromWitness

infix 6 _âˆ§_

_âˆ§_ : Bool â†’ Bool â†’ Bool
true âˆ§ true = true
false âˆ§ _   = false
_   âˆ§ false = false

infixr 6 _Ã—-dec_

_Ã—-dec_ : âˆ€ {A B : Set} â†’ Dec A â†’ Dec B â†’ Dec (A Ã— B)
yes a Ã—-dec yes b = yes âŸ¨ a , b âŸ©
no Â¬a Ã—-dec _     = no Î»{ âŸ¨ a , b âŸ© â†’ Â¬a a }
_     Ã—-dec no Â¬b = no Î»{ âŸ¨ a , b âŸ© â†’ Â¬b b }

infixr 5 _âˆ¨_

_âˆ¨_ : Bool â†’ Bool â†’ Bool
true  âˆ¨ _      = true
_     âˆ¨ true   = true
false âˆ¨ false  = false

infixr 5 _âŠ-dec_

_âŠ-dec_ : âˆ€ {A B : Set} â†’ Dec A â†’ Dec B â†’ Dec (A âŠ B)

yes a âŠ-dec _     = yes (injâ‚ a)
_     âŠ-dec yes b = yes (injâ‚‚ b)
no Â¬a âŠ-dec no Â¬b = no Î»{ (injâ‚ a) â†’ Â¬a a ; (injâ‚‚ b) â†’ Â¬b b }

not : Bool â†’ Bool
not true  = false
not false = true

Â¬? : âˆ€ {A : Set} â†’ Dec A â†’ Dec (Â¬ A)
Â¬? (yes a) = no (Â¬Â¬-intro a)
Â¬? (no Â¬a) = yes Â¬a

_âŠƒ_ : Bool â†’ Bool â†’ Bool
_     âŠƒ true     = true
false âŠƒ _    = true
true  âŠƒ false = false

_â†’-dec_ : âˆ€ {A B : Set} â†’ Dec A â†’ Dec B â†’ Dec (A â†’ B)
_     â†’-dec yes b = yes Î» { _ â†’ b }
no Â¬a â†’-dec no Â¬b = yes Î»{ a â†’ âŠ¥-elim (Â¬a a) }
yes a â†’-dec no Â¬b = no Î» { aâ†’b â†’ Â¬b (aâ†’b a) }

âˆ§-Ã— : âˆ€ {A B : Set} (x : Dec A) (y : Dec B) â†’ âŒŠ x âŒ‹ âˆ§ âŒŠ y âŒ‹ â‰¡ âŒŠ x Ã—-dec y âŒ‹
âˆ§-Ã— (yes a) (yes b) = refl
âˆ§-Ã— (no Â¬a) _       = refl
âˆ§-Ã— (yes a) (no Â¬b) = refl

âˆ¨-âŠ : âˆ€ {A B : Set} (x : Dec A) (y : Dec B) â†’ âŒŠ x âŒ‹ âˆ¨ âŒŠ y âŒ‹ â‰¡ âŒŠ x âŠ-dec y âŒ‹
âˆ¨-âŠ (yes a) _       = refl
âˆ¨-âŠ (no Â¬a) (yes b) = refl
âˆ¨-âŠ (no Â¬a) (no Â¬b) = refl

not-Â¬ : âˆ€ {A : Set} (x : Dec A) â†’ not âŒŠ x âŒ‹ â‰¡ âŒŠ Â¬? x âŒ‹
not-Â¬ (yes a) = refl
not-Â¬ (no Â¬a) = refl

_iff_ : Bool â†’ Bool â†’ Bool
true  iff true  = true
false iff true  = false
true  iff false = false
false iff false = true

_â‡”-dec_ : âˆ€ {A B : Set} â†’ Dec A â†’ Dec B â†’ Dec (A â‡” B)
yes a â‡”-dec yes b = yes record { to = Î»{ _ â†’ b} ; from  = Î»{ _ â†’ a} }
yes a â‡”-dec no Â¬b = no Î»{ aâ‡”b â†’ Â¬b (_â‡”_.to aâ‡”b a)}
no Â¬a â‡”-dec yes b = no Î»{ aâ‡”b â†’ Â¬a (_â‡”_.from aâ‡”b b)}
no Â¬a â‡”-dec no Â¬b = yes record { to = Î» { a â†’ âŠ¥-elim (Â¬a a) } ; from = Î» { b â†’ âŠ¥-elim (Â¬b b) } }

iff-â‡” : âˆ€ {A B : Set} (x : Dec A) (y : Dec B) â†’ âŒŠ x âŒ‹ iff âŒŠ y âŒ‹ â‰¡ âŒŠ x â‡”-dec y âŒ‹
iff-â‡” (yes a) (yes b) = refl
iff-â‡” (yes a) (no Â¬b) = refl
iff-â‡” (no Â¬a) (yes b) = refl
iff-â‡” (no Â¬a) (no Â¬b) = refl
